feat: redefine HashSet.union and add lemmas (#10611)
This PR adds adds union operation on `DHashMap`/`HashMap`/`HashSet` and
their raw variants and provides lemmas about union operations.

---------

Co-authored-by: Paul-Lez <paul.lezeau@gmail.com>
Co-authored-by: Markus Himmel <markus@lean-fro.org>
Co-authored-by: Markus Himmel <markus@himmel-villmar.de>

src/Std/Data/DHashMap/Internal/Defs.lean
@@ -426,6 +426,20 @@ def insertMany {ρ : Type w} [ForIn Id ρ ((a : α) × β a)] [BEq α] [Hashable
     r := ⟨r.1.insert a b, fun _ h hm => h (r.2 _ h hm)⟩
   return r
 
+/-- Internal implementation detail of the hash map -/
+@[inline] def insertManyIfNew {ρ : Type w} [ForIn Id ρ ((a : α) × β a)] [BEq α] [Hashable α]
+    (m : Raw₀ α β) (l : ρ) : { m' : Raw₀ α β // ∀ (P : Raw₀ α β → Prop),
+      (∀ {m'' a b}, P m'' → P (m''.insertIfNew a b)) → P m → P m' } := Id.run do
+  let mut r : { m' : Raw₀ α β // ∀ (P : Raw₀ α β → Prop),
+    (∀ {m'' a b}, P m'' → P (m''.insertIfNew a b)) → P m → P m' } := ⟨m, fun _ _ => id⟩
+  for ⟨a, b⟩ in l do
+    r := ⟨r.1.insertIfNew a b, fun _ h hm => h (r.2 _ h hm)⟩
+  return r
+
+/-- Internal implementation detail of the hash map -/
+@[inline] def union [BEq α] [Hashable α] (m₁ m₂ : Raw₀ α β) : Raw₀ α β :=
+  if m₁.1.size ≤ m₂.1.size then (m₂.insertManyIfNew m₁.1).1 else (m₁.insertMany m₂.1).1
+
 section
 
 variable {β : Type v}
