src/Std/Data/DHashMap/Lemmas.lean
@@ -64,6 +64,11 @@ theorem mem_iff_contains {a : α} : a ∈ m ↔ m.contains a :=
 theorem contains_iff_mem {a : α} : m.contains a ↔ a ∈ m :=
   Iff.rfl
 
+-- The following lemma becomes a simp lemma at the bottom of the file.
+theorem contains_eq_false_iff_not_mem {k : α} : m.contains k = false ↔ ¬k ∈ m := by
+  rw [← Bool.not_eq_true]
+  simp only [contains_iff_mem]
+
 theorem contains_congr [EquivBEq α] [LawfulHashable α] {a b : α} (hab : a == b) :
     m.contains a = m.contains b :=
   Raw₀.contains_congr _ m.2 hab
@@ -1765,6 +1770,299 @@ theorem isEmpty_insertMany_list [EquivBEq α] [LawfulHashable α]
 theorem isEmpty_of_isEmpty_insertMany [EquivBEq α] [LawfulHashable α]
     {l : ρ} : (m.insertMany l).isEmpty → m.isEmpty :=
   Raw₀.isEmpty_of_isEmpty_insertMany ⟨m.1, _⟩ m.2
+
+section Union
+
+variable (m₁ m₂ : DHashMap α β)
+
+variable {m₁ m₂}
+
+@[simp]
+theorem union_eq : m₁.union m₂ = m₁ ∪ m₂ := by
+  simp only [Union.union]
+
+/- contains -/
+@[simp]
+theorem contains_union [EquivBEq α] [LawfulHashable α]
+    {k : α} :
+    (m₁ ∪ m₂).contains k = (m₁.contains k || m₂.contains k) :=
+  @Raw₀.contains_union _ _ _ _ ⟨m₁.1, m₁.2.size_buckets_pos⟩ ⟨m₂.1, m₂.2.size_buckets_pos⟩ _ _ m₁.2 m₂.2 k
+
+/- mem -/
+theorem mem_union_of_left [EquivBEq α] [LawfulHashable α] {k : α} :
+    k ∈ m₁ → k ∈ m₁ ∪ m₂ :=
+  @Raw₀.contains_union_of_left _ _ _ _ ⟨m₁.1, _⟩ ⟨m₂.1, _⟩ _ _ m₁.2 m₂.2 k
+
+theorem mem_union_of_right [EquivBEq α] [LawfulHashable α] {k : α} :
+    k ∈ m₂ → k ∈ m₁ ∪ m₂ :=
+  @Raw₀.contains_union_of_right _ _ _ _ ⟨m₁.1, _⟩ ⟨m₂.1, _⟩ _ _ m₁.2 m₂.2 k
+
+@[simp]
+theorem mem_union_iff [EquivBEq α] [LawfulHashable α] {k : α} :
+    k ∈ m₁ ∪ m₂ ↔ k ∈ m₁ ∨ k ∈ m₂ :=
+  @Raw₀.contains_union_iff _ _ _ _ ⟨m₁.1, _⟩ ⟨m₂.1, _⟩ _ _ m₁.2 m₂.2 k
+
+theorem mem_of_mem_union_of_not_mem_right [EquivBEq α]
+    [LawfulHashable α] {k : α} :
+    k ∈ m₁ ∪ m₂ → ¬k ∈ m₂ → k ∈ m₁ := by
+  intro h₁ h₂
+  rw [← contains_eq_false_iff_not_mem] at h₂
+  exact @Raw₀.contains_of_contains_union_of_contains_eq_false_right _ _ _ _ ⟨m₁.1, m₁.2.size_buckets_pos⟩ ⟨m₂.1, m₂.2.size_buckets_pos⟩ _ _ m₁.2 m₂.2 k h₁ h₂
+
+theorem mem_of_mem_union_of_not_mem_left [EquivBEq α]
+    [LawfulHashable α] {k : α} :
+    k ∈ m₁ ∪ m₂ → ¬k ∈ m₁ → k ∈ m₂ := by
+  intro h₁ h₂
+  rw [← contains_eq_false_iff_not_mem] at h₂
+  exact @Raw₀.contains_of_contains_union_of_contains_eq_false_left _ _ _ _ ⟨m₁.1, _⟩ ⟨m₂.1, _⟩ _ _ m₁.2 m₂.2 k h₁ h₂
+
+/- Equiv -/
+theorem union_insert_right_equiv_union_insert [EquivBEq α] [LawfulHashable α] {p : (a : α) × β a} :
+    (m₁ ∪ (m₂.insert p.fst p.snd)) ~m ((m₁ ∪ m₂).insert p.fst p.snd) :=
+  ⟨@Raw₀.union_insert_right_equiv_insert_union _ _ _ _ ⟨m₁.1, m₁.2.size_buckets_pos⟩ ⟨m₂.1, m₂.2.size_buckets_pos⟩ _ _ p m₁.2 m₂.2⟩
+
+/- get? -/
+theorem get?_union [LawfulBEq α] {k : α} :
+    (m₁ ∪ m₂).get? k = (m₂.get? k).or (m₁.get? k) :=
+  @Raw₀.get?_union _ _ _ _ ⟨m₁.1, m₁.2.size_buckets_pos⟩ ⟨m₂.1, m₂.2.size_buckets_pos⟩ _ m₁.2 m₂.2 k
+
+theorem get?_union_of_not_mem_left [LawfulBEq α]
+    {k : α} (not_mem : ¬k ∈ m₁) :
+    (m₁ ∪ m₂).get? k = m₂.get? k := by
+  rw [← contains_eq_false_iff_not_mem] at not_mem
+  exact @Raw₀.get?_union_of_contains_eq_false_left _ _ _ _ ⟨m₁.1, m₁.2.size_buckets_pos⟩ ⟨m₂.1, m₂.2.size_buckets_pos⟩ _ m₁.2 m₂.2 k not_mem
+
+theorem get?_union_of_not_mem_right [LawfulBEq α]
+    {k : α} (not_mem : ¬k ∈ m₂) :
+    (m₁ ∪ m₂).get? k = m₁.get? k := by
+  rw [← contains_eq_false_iff_not_mem] at not_mem
+  exact @Raw₀.get?_union_of_contains_eq_false_right _ _ _ _ ⟨m₁.1, m₁.2.size_buckets_pos⟩ ⟨m₂.1, m₂.2.size_buckets_pos⟩ _ m₁.2 m₂.2 k not_mem
+
+/- get -/
+theorem get_union_of_mem_right [LawfulBEq α]
+    {k : α} (mem : k ∈ m₂) :
+    (m₁ ∪ m₂).get k (mem_union_of_right mem) = m₂.get k mem :=
+  @Raw₀.get_union_of_contains_right _ _ _ _ ⟨m₁.1, _⟩ ⟨m₂.1, _⟩ _ m₁.2 m₂.2 k mem
+
+theorem get_union_of_not_mem_left [LawfulBEq α]
+    {k : α} (not_mem : ¬k ∈ m₁) {h'} :
+    (m₁ ∪ m₂).get k h' = m₂.get k (mem_of_mem_union_of_not_mem_left h' not_mem) := by
+  rw [← contains_eq_false_iff_not_mem] at not_mem
+  rw [mem_iff_contains] at h'
+  exact @Raw₀.get_union_of_contains_eq_false_left _ _ _ _ ⟨m₁.1, _⟩ ⟨m₂.1, m₂.2.size_buckets_pos⟩ _ m₁.2 m₂.2 k not_mem h'
+
+theorem get_union_of_not_mem_right [LawfulBEq α]
+    {k : α} (not_mem : ¬k ∈ m₂) {h'} :
+    (m₁ ∪ m₂).get k h' = m₁.get k (mem_of_mem_union_of_not_mem_right h' not_mem) := by
+  rw [← contains_eq_false_iff_not_mem] at not_mem
+  rw [mem_iff_contains] at h'
+  exact @Raw₀.get_union_of_contains_eq_false_right _ _ _ _ ⟨m₁.1, _⟩ ⟨m₂.1, m₂.2.size_buckets_pos⟩ _ m₁.2 m₂.2 k not_mem h'
+
+/- getD -/
+theorem getD_union [LawfulBEq α] {k : α} {fallback : β k} :
+    (m₁ ∪ m₂).getD k fallback = m₂.getD k (m₁.getD k fallback) :=
+  @Raw₀.getD_union _ _ _ _ ⟨m₁.1, m₁.2.size_buckets_pos⟩ ⟨m₂.1, m₂.2.size_buckets_pos⟩ _ m₁.2 m₂.2 k fallback
+
+theorem getD_union_of_not_mem_left [LawfulBEq α]
+    {k : α} {fallback : β k} (not_mem : ¬k ∈ m₁) :
+    (m₁ ∪ m₂).getD k fallback = m₂.getD k fallback := by
+  rw [← contains_eq_false_iff_not_mem] at not_mem
+  exact @Raw₀.getD_union_of_contains_eq_false_left _ _ _ _ ⟨m₁.1, m₁.2.size_buckets_pos⟩ ⟨m₂.1, m₂.2.size_buckets_pos⟩ _ m₁.2 m₂.2 k fallback not_mem
+
+theorem getD_union_of_not_mem_right [LawfulBEq α]
+    {k : α} {fallback : β k} (not_mem : ¬k ∈ m₂)  :
+    (m₁ ∪ m₂).getD k fallback = m₁.getD k fallback := by
+  rw [← contains_eq_false_iff_not_mem] at not_mem
+  exact @Raw₀.getD_union_of_contains_eq_false_right _ _ _ _ ⟨m₁.1, m₁.2.size_buckets_pos⟩ ⟨m₂.1, m₂.2.size_buckets_pos⟩ _ m₁.2 m₂.2 k fallback not_mem
+
+/- get! -/
+theorem get!_union [LawfulBEq α] {k : α} [Inhabited (β k)] :
+    (m₁ ∪ m₂).get! k = m₂.getD k (m₁.get! k) :=
+  @Raw₀.get!_union _ _ _ _ ⟨m₁.1, m₁.2.size_buckets_pos⟩ ⟨m₂.1, m₂.2.size_buckets_pos⟩ _ m₁.2 m₂.2 k _
+
+theorem get!_union_of_not_mem_left [LawfulBEq α]
+    {k : α} [Inhabited (β k)] (not_mem : ¬k ∈ m₁) :
+    (m₁ ∪ m₂).get! k = m₂.get! k := by
+  rw [← contains_eq_false_iff_not_mem] at not_mem
+  exact @Raw₀.get!_union_of_contains_eq_false_left _ _ _ _ ⟨m₁.1, m₁.2.size_buckets_pos⟩ ⟨m₂.1, m₂.2.size_buckets_pos⟩ _ m₁.2 m₂.2 k _ not_mem
+
+theorem get!_union_of_not_mem_right [LawfulBEq α]
+    {k : α} [Inhabited (β k)] (not_mem : ¬k ∈ m₂)  :
+    (m₁ ∪ m₂).get! k = m₁.get! k := by
+  rw [← contains_eq_false_iff_not_mem] at not_mem
+  exact @Raw₀.get!_union_of_contains_eq_false_right _ _ _ _ ⟨m₁.1, m₁.2.size_buckets_pos⟩ ⟨m₂.1, m₂.2.size_buckets_pos⟩ _ m₁.2 m₂.2 k _ not_mem
+
+/- getKey? -/
+theorem getKey?_union [EquivBEq α] [LawfulHashable α] {k : α} :
+    (m₁ ∪ m₂).getKey? k = (m₂.getKey? k).or (m₁.getKey? k) :=
+  @Raw₀.getKey?_union _ _ _ _ ⟨m₁.1, m₁.2.size_buckets_pos⟩ ⟨m₂.1, m₂.2.size_buckets_pos⟩ _ _ m₁.2 m₂.2 k
+
+theorem getKey?_union_of_not_mem_left [EquivBEq α] [LawfulHashable α]
+    {k : α} (not_mem : ¬k ∈ m₁) :
+    (m₁ ∪ m₂).getKey? k = m₂.getKey? k := by
+  rw [← contains_eq_false_iff_not_mem] at not_mem
+  exact @Raw₀.getKey?_union_of_contains_eq_false_left _ _ _ _ ⟨m₁.1, m₁.2.size_buckets_pos⟩ ⟨m₂.1, m₂.2.size_buckets_pos⟩ _ _ m₁.2 m₂.2 k not_mem
+
+theorem getKey?_union_of_not_mem_right [EquivBEq α] [LawfulHashable α]
+    {k : α} (not_mem : ¬k ∈ m₂) :
+    (m₁ ∪ m₂).getKey? k = m₁.getKey? k := by
+  rw [← contains_eq_false_iff_not_mem] at not_mem
+  exact @Raw₀.getKey?_union_of_contains_eq_false_right _ _ _ _ ⟨m₁.1, m₁.2.size_buckets_pos⟩ ⟨m₂.1, m₂.2.size_buckets_pos⟩ _ _ m₁.2 m₂.2 k not_mem
+
+/- getKey -/
+theorem getKey_union_of_mem_right [EquivBEq α] [LawfulHashable α]
+    {k : α} (mem : k ∈ m₂) :
+    (m₁ ∪ m₂).getKey k (mem_union_of_right mem) = m₂.getKey k mem :=
+  @Raw₀.getKey_union_of_contains_right _ _ _ _ ⟨m₁.1, _⟩ ⟨m₂.1, _⟩ _ _ m₁.2 m₂.2 k mem
+
+theorem getKey_union_of_not_mem_left [EquivBEq α] [LawfulHashable α]
+    {k : α} (not_mem : ¬k ∈ m₁) {h'} :
+    (m₁ ∪ m₂).getKey k h' = m₂.getKey k (mem_of_mem_union_of_not_mem_left h' not_mem) :=by
+  rw [← contains_eq_false_iff_not_mem] at not_mem
+  exact @Raw₀.getKey_union_of_contains_eq_false_left _ _ _ _ ⟨m₁.1, m₁.2.size_buckets_pos⟩ ⟨m₂.1, m₂.2.size_buckets_pos⟩ _ _ m₁.2 m₂.2 k not_mem h'
+
+theorem getKey_union_of_not_mem_right [EquivBEq α] [LawfulHashable α]
+    {k : α} (not_mem : ¬k ∈ m₂) {h'} :
+    (m₁ ∪ m₂).getKey k h' = m₁.getKey k (mem_of_mem_union_of_not_mem_right h' not_mem) := by
+  rw [← contains_eq_false_iff_not_mem] at not_mem
+  exact @Raw₀.getKey_union_of_contains_eq_false_right _ _ _ _ ⟨m₁.1, m₁.2.size_buckets_pos⟩ ⟨m₂.1, m₂.2.size_buckets_pos⟩ _ _ m₁.2 m₂.2 k not_mem h'
+
+/- getKeyD -/
+theorem getKeyD_union [EquivBEq α] [LawfulHashable α] {k fallback : α} :
+    (m₁ ∪ m₂).getKeyD k fallback = m₂.getKeyD k (m₁.getKeyD k fallback) :=
+  @Raw₀.getKeyD_union _ _ _ _ ⟨m₁.1, m₁.2.size_buckets_pos⟩ ⟨m₂.1, m₂.2.size_buckets_pos⟩ _ _ m₁.2 m₂.2 k fallback
+
+theorem getKeyD_union_of_not_mem_left [EquivBEq α] [LawfulHashable α]
+    {k fallback : α} (not_mem : ¬k ∈ m₁) :
+    (m₁ ∪ m₂).getKeyD k fallback = m₂.getKeyD k fallback :=by
+  rw [← contains_eq_false_iff_not_mem] at not_mem
+  exact @Raw₀.getKeyD_union_of_contains_eq_false_left _ _ _ _ ⟨m₁.1, m₁.2.size_buckets_pos⟩ ⟨m₂.1, m₂.2.size_buckets_pos⟩ _ _ m₁.2 m₂.2 k fallback not_mem
+
+theorem getKeyD_union_of_not_mem_right [EquivBEq α] [LawfulHashable α]
+    {k fallback : α} (not_mem : ¬k ∈ m₂) :
+    (m₁ ∪ m₂).getKeyD k fallback = m₁.getKeyD k fallback := by
+  rw [← contains_eq_false_iff_not_mem] at not_mem
+  exact @Raw₀.getKeyD_union_of_contains_eq_false_right _ _ _ _ ⟨m₁.1, m₁.2.size_buckets_pos⟩ ⟨m₂.1, m₂.2.size_buckets_pos⟩ _ _ m₁.2 m₂.2 k fallback not_mem
+
+/- getKey! -/
+theorem getKey!_union [EquivBEq α] [LawfulHashable α] [Inhabited α] {k : α} :
+    (m₁ ∪ m₂).getKey! k = m₂.getKeyD k (m₁.getKey! k) :=
+  @Raw₀.getKey!_union _ _ _ _ ⟨m₁.1, m₁.2.size_buckets_pos⟩ ⟨m₂.1, m₂.2.size_buckets_pos⟩ _ _ _ m₁.2 m₂.2 k
+
+theorem getKey!_union_of_not_mem_left [Inhabited α]
+    [EquivBEq α] [LawfulHashable α] {k : α}
+    (not_mem : ¬k ∈ m₁) :
+    (m₁ ∪ m₂).getKey! k = m₂.getKey! k := by
+  rw [← contains_eq_false_iff_not_mem] at not_mem
+  exact @Raw₀.getKey!_union_of_contains_eq_false_left _ _ _ _ ⟨m₁.1, m₁.2.size_buckets_pos⟩ ⟨m₂.1, m₂.2.size_buckets_pos⟩ _ _ _ m₁.2 m₂.2 k not_mem
+
+theorem getKey!_union_of_not_mem_right [Inhabited α]
+    [EquivBEq α] [LawfulHashable α] {k : α}
+    (not_mem : ¬k ∈ m₂) :
+    (m₁ ∪ m₂).getKey! k = m₁.getKey! k := by
+  rw [← contains_eq_false_iff_not_mem] at not_mem
+  exact @Raw₀.getKey!_union_of_contains_eq_false_right _ _ _ _ ⟨m₁.1, m₁.2.size_buckets_pos⟩ ⟨m₂.1, m₂.2.size_buckets_pos⟩ _ _ _ m₁.2 m₂.2 k not_mem
+
+/- size -/
+theorem size_union_of_not_mem [EquivBEq α] [LawfulHashable α] :
+    (∀ (a : α), a ∈ m₁ → ¬a ∈ m₂) →
+    (m₁ ∪ m₂).size = m₁.size + m₂.size := by
+  simp only [← contains_eq_false_iff_not_mem]
+  exact @Raw₀.size_union_of_not_mem _ _ _ _ ⟨m₁.1, m₁.2.size_buckets_pos⟩ ⟨m₂.1, m₂.2.size_buckets_pos⟩ _ _ m₁.2 m₂.2
+
+theorem size_left_le_size_union [EquivBEq α] [LawfulHashable α] : m₁.size ≤ (m₁ ∪ m₂).size :=
+  @Raw₀.size_left_le_size_union α β _ _ ⟨m₁.1, m₁.2.size_buckets_pos⟩ ⟨m₂.1, m₂.2.size_buckets_pos⟩ _ _ m₁.2 m₂.2
+
+theorem size_right_le_size_union [EquivBEq α] [LawfulHashable α] :
+    m₂.size ≤ (m₁ ∪ m₂).size :=
+  @Raw₀.size_right_le_size_union _ _ _ _ ⟨m₁.1, m₁.2.size_buckets_pos⟩ ⟨m₂.1, m₂.2.size_buckets_pos⟩ _ _ m₁.2 m₂.2
+
+theorem size_union_le_size_add_size [EquivBEq α] [LawfulHashable α] :
+    (m₁ ∪ m₂).size ≤ m₁.size + m₂.size :=
+  @Raw₀.size_union_le_size_add_size _ _ _ _ ⟨m₁.1, m₁.2.size_buckets_pos⟩ ⟨m₂.1, m₂.2.size_buckets_pos⟩ _ _ m₁.2 m₂.2
+
+/- isEmpty -/
+@[simp]
+theorem isEmpty_union [EquivBEq α] [LawfulHashable α] :
+    (m₁ ∪ m₂).isEmpty = (m₁.isEmpty && m₂.isEmpty) :=
+  @Raw₀.isEmpty_union α β _ _ ⟨m₁.1, m₁.2.size_buckets_pos⟩ ⟨m₂.1, m₂.2.size_buckets_pos⟩ _ _ m₁.2 m₂.2
+
+end Union
+
+namespace Const
+
+variable {β : Type v} {m₁ m₂ : DHashMap α (fun _ => β)}
+
+/- get? -/
+theorem get?_union [EquivBEq α] [LawfulHashable α] {k : α} :
+    Const.get? (m₁.union m₂) k = (Const.get? m₂ k).or (Const.get? m₁ k) :=
+  @Raw₀.Const.get?_union _ _ _ _ ⟨m₁.1, _⟩ ⟨m₂.1, _⟩ _ _ m₁.2 m₂.2 k
+
+theorem get?_union_of_not_mem_left [EquivBEq α] [LawfulHashable α]
+    {k : α} (not_mem : ¬k ∈ m₁) :
+    Const.get? (m₁.union m₂) k = Const.get? m₂ k := by
+  rw [← contains_eq_false_iff_not_mem] at not_mem
+  exact @Raw₀.Const.get?_union_of_contains_eq_false_left _ _ _ _ ⟨m₁.1, _⟩ ⟨m₂.1, _⟩ _ _ m₁.2 m₂.2 k not_mem
+
+theorem get?_union_of_not_mem_right [EquivBEq α] [LawfulHashable α]
+    {k : α} (not_mem : ¬k ∈ m₂) :
+    Const.get? (m₁.union m₂) k = Const.get? m₁ k := by
+  rw [← contains_eq_false_iff_not_mem] at not_mem
+  exact @Raw₀.Const.get?_union_of_contains_eq_false_right _ _ _ _ ⟨m₁.1, _⟩ ⟨m₂.1, _⟩ _ _ m₁.2 m₂.2 k not_mem
+
+/- get -/
+theorem get_union_of_mem_right [EquivBEq α] [LawfulHashable α]
+    {k : α} (mem : m₂.contains k) :
+    Const.get (m₁.union m₂) k (mem_union_of_right mem) = Const.get m₂ k mem :=
+  @Raw₀.Const.get_union_of_contains_right _ _ _ _ ⟨m₁.1, _⟩ ⟨m₂.1, _⟩ _ _  m₁.2 m₂.2 k mem
+
+theorem get_union_of_not_mem_left [EquivBEq α] [LawfulHashable α]
+    {k : α} (not_mem : ¬k ∈ m₁) {h'} :
+    Const.get (m₁.union m₂) k h' = Const.get m₂ k (mem_of_mem_union_of_not_mem_left h' not_mem) := by
+  rw [← contains_eq_false_iff_not_mem] at not_mem
+  exact @Raw₀.Const.get_union_of_contains_eq_false_left _ _ _ _ ⟨m₁.1, _⟩ ⟨m₂.1, _⟩ _ _  m₁.2 m₂.2 k not_mem h'
+
+theorem get_union_of_not_mem_right [EquivBEq α] [LawfulHashable α]
+    {k : α} (not_mem : ¬k ∈ m₂) {h'} :
+    Const.get (m₁.union m₂) k h' = Const.get m₁ k (mem_of_mem_union_of_not_mem_right h' not_mem) := by
+  rw [← contains_eq_false_iff_not_mem] at not_mem
+  exact @Raw₀.Const.get_union_of_contains_eq_false_right _ _ _ _ ⟨m₁.1, _⟩ ⟨m₂.1, _⟩ _ _  m₁.2 m₂.2 k not_mem h'
+
+/- getD -/
+theorem getD_union [EquivBEq α] [LawfulHashable α] {k : α} {fallback : β} :
+    Const.getD (m₁.union m₂) k fallback = Const.getD m₂ k (Const.getD m₁ k fallback) :=
+  @Raw₀.Const.getD_union _ _ _ _ ⟨m₁.1, m₁.2.size_buckets_pos⟩ ⟨m₂.1, m₂.2.size_buckets_pos⟩ _ _  m₁.2 m₂.2 k fallback
+
+theorem getD_union_of_not_mem_left [EquivBEq α] [LawfulHashable α]
+    {k : α} {fallback : β} (not_mem : ¬k ∈ m₁) :
+    Const.getD (m₁.union m₂) k fallback = Const.getD m₂ k fallback := by
+  rw [← contains_eq_false_iff_not_mem] at not_mem
+  exact @Raw₀.Const.getD_union_of_contains_eq_false_left _ _ _ _ ⟨m₁.1, m₁.2.size_buckets_pos⟩ ⟨m₂.1, m₂.2.size_buckets_pos⟩ _ _  m₁.2 m₂.2 k fallback not_mem
+
+theorem getD_union_of_not_mem_right [EquivBEq α] [LawfulHashable α]
+    {k : α} {fallback : β} (not_mem : ¬k ∈ m₂) :
+    Const.getD (m₁.union m₂) k fallback = Const.getD m₁ k fallback := by
+  rw [← contains_eq_false_iff_not_mem] at not_mem
+  exact @Raw₀.Const.getD_union_of_contains_eq_false_right _ _ _ _ ⟨m₁.1, m₁.2.size_buckets_pos⟩ ⟨m₂.1, m₂.2.size_buckets_pos⟩ _ _  m₁.2 m₂.2 k fallback not_mem
+
+/- get! -/
+theorem get!_union [EquivBEq α] [LawfulHashable α] [Inhabited β] {k : α} :
+    Const.get! (m₁.union m₂) k = Const.getD m₂ k (Const.get! m₁ k) :=
+  @Raw₀.Const.get!_union _ _ _ _ ⟨m₁.1, m₁.2.size_buckets_pos⟩ ⟨m₂.1, m₂.2.size_buckets_pos⟩ _ _ _ m₁.2 m₂.2 k
+
+theorem get!_union_of_not_mem_left [EquivBEq α] [LawfulHashable α] [Inhabited β]
+    {k : α} (not_mem : ¬k ∈ m₁) :
+    Const.get! (m₁.union m₂) k = Const.get! m₂ k := by
+  rw [← contains_eq_false_iff_not_mem] at not_mem
+  exact @Raw₀.Const.get!_union_of_contains_eq_false_left _ _ _ _ ⟨m₁.1, m₁.2.size_buckets_pos⟩ ⟨m₂.1, m₂.2.size_buckets_pos⟩ _ _ _  m₁.2 m₂.2 k not_mem
+
+theorem get!_union_of_not_mem_right [EquivBEq α] [LawfulHashable α] [Inhabited β]
+    {k : α} (not_mem : ¬k ∈ m₂) :
+    Const.get! (m₁.union m₂) k = Const.get! m₁ k := by
+  rw [← contains_eq_false_iff_not_mem] at not_mem
+  exact @Raw₀.Const.get!_union_of_contains_eq_false_right _ _ _ _ ⟨m₁.1, m₁.2.size_buckets_pos⟩ ⟨m₂.1, m₂.2.size_buckets_pos⟩ _ _ _  m₁.2 m₂.2 k not_mem
+
+end Const
 
 namespace Const
 
@@ -4273,5 +4571,5 @@ theorem toList_map {m : DHashMap α fun _ => β}
 end Const
 
 end map
-
+attribute [simp] contains_eq_false_iff_not_mem
 end Std.DHashMap
