src/Std/Data/HashSet/RawLemmas.lean
@@ -76,6 +76,10 @@ theorem mem_iff_contains {a : α} : a ∈ m ↔ m.contains a :=
 theorem contains_iff_mem {a : α} : m.contains a ↔ a ∈ m :=
   HashMap.Raw.contains_iff_mem
 
+-- The following lemma becomes a simp lemma at the bottom of the file.
+theorem contains_eq_false_iff_not_mem {k : α} : m.contains k = false ↔ ¬k ∈ m :=
+  HashMap.Raw.contains_eq_false_iff_not_mem
+
 theorem contains_congr [EquivBEq α] [LawfulHashable α] (h : m.WF) {a b : α} (hab : a == b) :
     m.contains a = m.contains b :=
   HashMap.Raw.contains_congr h.out hab
@@ -773,6 +777,149 @@ theorem isEmpty_of_isEmpty_insertMany [EquivBEq α] [LawfulHashable α] (h : m.W
     {l : ρ} : (insertMany m l).isEmpty → m.isEmpty :=
   HashMap.Raw.isEmpty_of_isEmpty_insertManyIfNewUnit h.out
 
+section Union
+
+variable (m₁ m₂ : Raw α)
+
+variable {m₁ m₂}
+
+@[simp]
+theorem union_eq : m₁.union m₂ = m₁ ∪ m₂ := by
+  simp only [Union.union]
+
+/- contains -/
+@[simp]
+theorem contains_union [EquivBEq α] [LawfulHashable α] (h₁ : m₁.WF)
+    (h₂ : m₂.WF) {k : α} :
+    (m₁ ∪ m₂).contains k = (m₁.contains k || m₂.contains k) :=
+  @HashMap.Raw.contains_union _ _ _ _ m₁.inner m₂.inner _ _ h₁.out h₂.out k
+
+/- mem -/
+theorem mem_union_of_left [EquivBEq α] [LawfulHashable α] (h₁ : m₁.WF)
+    (h₂ : m₂.WF) {k : α} :
+    k ∈ m₁ → k ∈ m₁ ∪ m₂ :=
+  @HashMap.Raw.mem_union_of_left _ _ _ _ m₁.inner m₂.inner _ _ h₁.out h₂.out k
+
+theorem mem_union_of_right [EquivBEq α] [LawfulHashable α] (h₁ : m₁.WF)
+    (h₂ : m₂.WF) {k : α} :
+    k ∈ m₂ → k ∈ m₁ ∪ m₂ :=
+  @HashMap.Raw.mem_union_of_right _ _ _ _ m₁.inner m₂.inner _ _ h₁.out h₂.out k
+
+@[simp]
+theorem mem_union_iff [EquivBEq α] [LawfulHashable α] (h₁ : m₁.WF)
+    (h₂ : m₂.WF) {k : α} :
+    k ∈ m₁ ∪ m₂ ↔ k ∈ m₁ ∨ k ∈ m₂ :=
+  @HashMap.Raw.mem_union_iff _ _ _ _ m₁.inner m₂.inner _ _ h₁.out h₂.out k
+
+theorem mem_of_mem_union_of_not_mem_right [EquivBEq α]
+    [LawfulHashable α] (h₁ : m₁.WF) (h₂ : m₂.WF) {k : α} :
+    k ∈ m₁ ∪ m₂ → ¬k ∈ m₂ → k ∈ m₁ :=
+  @HashMap.Raw.mem_of_mem_union_of_not_mem_right _ _ _ _ m₁.inner m₂.inner _ _ h₁.out h₂.out k
+
+theorem mem_of_mem_union_of_not_mem_left [EquivBEq α]
+    [LawfulHashable α] (h₁ : m₁.WF) (h₂ : m₂.WF) {k : α} :
+    k ∈ m₁ ∪ m₂ → ¬k ∈ m₁ → k ∈ m₂ :=
+  @HashMap.Raw.mem_of_mem_union_of_not_mem_left _ _ _ _ m₁.inner m₂.inner _ _ h₁.out h₂.out k
+
+/- get? -/
+theorem get?_union [EquivBEq α] [LawfulHashable α]
+    (h₁ : m₁.WF) (h₂ : m₂.WF)
+    {k : α} :
+    (m₁ ∪ m₂).get? k = (m₂.get? k).or (m₁.get? k) :=
+  @HashMap.Raw.getKey?_union _ _ _ _ m₁.inner m₂.inner _ _ h₁.out h₂.out k
+
+theorem get?_union_of_not_mem_left [EquivBEq α] [LawfulHashable α]
+    (h₁ : m₁.WF) (h₂ : m₂.WF)
+    {k : α} (not_mem : ¬k ∈ m₁) :
+    (m₁ ∪ m₂).get? k = m₂.get? k :=
+  @HashMap.Raw.getKey?_union_of_not_mem_left _ _ _ _ m₁.inner m₂.inner _ _ h₁.out h₂.out k not_mem
+
+theorem get?_union_of_not_mem_right [EquivBEq α] [LawfulHashable α]
+    (h₁ : m₁.WF) (h₂ : m₂.WF)
+    {k : α} (not_mem : ¬k ∈ m₂) :
+    (m₁ ∪ m₂).get? k = m₁.get? k :=
+  @HashMap.Raw.getKey?_union_of_not_mem_right _ _ _ _ m₁.inner m₂.inner _ _ h₁.out h₂.out k not_mem
+
+/- get -/
+theorem get_union_of_mem_right [EquivBEq α] [LawfulHashable α] (h₁ : m₁.WF) (h₂ : m₂.WF)
+    {k : α} (mem : k ∈ m₂) :
+    (m₁ ∪ m₂).get k (mem_union_of_right h₁ h₂ mem) = m₂.get k mem :=
+  @HashMap.Raw.getKey_union_of_mem_right _ _ _ _ m₁.inner m₂.inner _ _ h₁.out h₂.out k mem
+
+theorem get_union_of_not_mem_left [EquivBEq α] [LawfulHashable α] (h₁ : m₁.WF) (h₂ : m₂.WF)
+    {k : α} (not_mem : ¬k ∈ m₁) {h'} :
+    (m₁ ∪ m₂).get k h' = m₂.get k (mem_of_mem_union_of_not_mem_left h₁ h₂ h' not_mem) :=
+  @HashMap.Raw.getKey_union_of_not_mem_left _ _ _ _ m₁.inner m₂.inner _ _ h₁.out h₂.out k not_mem h'
+
+theorem get_union_of_not_mem_right [EquivBEq α] [LawfulHashable α] (h₁ : m₁.WF) (h₂ : m₂.WF)
+    {k : α} (not_mem : ¬k ∈ m₂) {h'} :
+    (m₁ ∪ m₂).get k h' = m₁.get k (mem_of_mem_union_of_not_mem_right h₁ h₂ h' not_mem) :=
+  @HashMap.Raw.getKey_union_of_not_mem_right _ _ _ _ m₁.inner m₂.inner _ _ h₁.out h₂.out k not_mem h'
+
+/- getD -/
+theorem getD_union [EquivBEq α]
+    [LawfulHashable α] (h₁ : m₁.WF)
+    (h₂ : m₂.WF) {k fallback : α} :
+    (m₁ ∪ m₂).getD k fallback = m₂.getD k (m₁.getD k fallback) :=
+  @HashMap.Raw.getKeyD_union _ _ _ _ m₁.inner m₂.inner _ _ h₁.out h₂.out k fallback
+
+theorem getD_union_of_not_mem_left [EquivBEq α] [LawfulHashable α] (h₁ : m₁.WF)
+    (h₂ : m₂.WF) {k fallback : α} (not_mem : ¬k ∈ m₁) :
+    (m₁ ∪ m₂).getD k fallback = m₂.getD k fallback :=
+  @HashMap.Raw.getKeyD_union_of_not_mem_left _ _ _ _ m₁.inner m₂.inner _ _ h₁.out h₂.out k fallback not_mem
+
+theorem getD_union_of_not_mem_right [EquivBEq α] [LawfulHashable α] (h₁ : m₁.WF)
+    (h₂ : m₂.WF) {k fallback : α} (not_mem : ¬k ∈ m₂) :
+    (m₁ ∪ m₂).getD k fallback = m₁.getD k fallback :=
+  @HashMap.Raw.getKeyD_union_of_not_mem_right _ _ _ _ m₁.inner m₂.inner _ _ h₁.out h₂.out k fallback not_mem
+
+/- get! -/
+theorem get!_union [EquivBEq α] [LawfulHashable α] [Inhabited α]
+    (h₁ : m₁.WF)
+    (h₂ : m₂.WF) {k : α} :
+    (m₁ ∪ m₂).get! k = m₂.getD k (m₁.get! k) :=
+  @HashMap.Raw.getKey!_union _ _ _ _ m₁.inner m₂.inner _ _ _ h₁.out h₂.out k
+
+theorem get!_union_of_not_mem_left [Inhabited α]
+    [EquivBEq α] [LawfulHashable α] (h₁ : m₁.WF) (h₂ : m₂.WF) {k : α}
+    (not_mem : ¬k ∈ m₁) :
+    (m₁ ∪ m₂).get! k = m₂.get! k :=
+  @HashMap.Raw.getKey!_union_of_not_mem_left _ _ _ _ m₁.inner m₂.inner _ _ _ h₁.out h₂.out k not_mem
+
+theorem get!_union_of_not_mem_right [Inhabited α]
+    [EquivBEq α] [LawfulHashable α] (h₁ : m₁.WF) (h₂ : m₂.WF) {k : α}
+    (not_mem : ¬k ∈ m₂) :
+    (m₁ ∪ m₂).get! k = m₁.get! k :=
+   @HashMap.Raw.getKey!_union_of_not_mem_right _ _ _ _ m₁.inner m₂.inner _ _ _ h₁.out h₂.out k not_mem
+
+/- size -/
+theorem size_union_of_not_mem [EquivBEq α] [LawfulHashable α] (h₁ : m₁.WF)
+    (h₂ : m₂.WF) : (∀ (a : α), a ∈ m₁ → ¬a ∈ m₂) →
+    (m₁ ∪ m₂).size = m₁.size + m₂.size :=
+  @HashMap.Raw.size_union_of_not_mem _ _ _ _ m₁.inner m₂.inner _ _ h₁.out h₂.out
+
+theorem size_left_le_size_union [EquivBEq α] [LawfulHashable α] (h₁ : m₁.WF)
+    (h₂ : m₂.WF) : m₁.size ≤ (m₁ ∪ m₂).size :=
+  @HashMap.Raw.size_left_le_size_union _ _ _ _ m₁.inner m₂.inner _ _ h₁.out h₂.out
+
+theorem size_right_le_size_union [EquivBEq α] [LawfulHashable α] (h₁ : m₁.WF)
+    (h₂ : m₂.WF) : m₂.size ≤ (m₁ ∪ m₂).size :=
+  @HashMap.Raw.size_right_le_size_union _ _ _ _ m₁.inner m₂.inner _ _ h₁.out h₂.out
+
+theorem size_union_le_size_add_size [EquivBEq α] [LawfulHashable α]
+    (h₁ : m₁.WF) (h₂ : m₂.WF) :
+    (m₁ ∪ m₂).size ≤ m₁.size + m₂.size :=
+  @HashMap.Raw.size_union_le_size_add_size _ _ _ _ m₁.inner m₂.inner _ _ h₁.out h₂.out
+
+/- isEmpty -/
+@[simp]
+theorem isEmpty_union [EquivBEq α] [LawfulHashable α] (h₁ : m₁.WF) (h₂ : m₂.WF) :
+    (m₁ ∪ m₂).isEmpty = (m₁.isEmpty && m₂.isEmpty) :=
+  @HashMap.Raw.isEmpty_union _ _ _ _ m₁.inner m₂.inner _ _ h₁.out h₂.out
+
+
+end Union
+
 @[simp, grind =]
 theorem ofList_nil :
     ofList ([] : List α) = ∅ :=
@@ -1053,6 +1200,7 @@ theorem get_filter [EquivBEq α] [LawfulHashable α]
 
 end filter
 
+attribute [simp] contains_eq_false_iff_not_mem
 end Raw
 
 end Std.HashSet
